BFS refinement partially done

Set_Graphs/Graph_Algorithms/BFS_Refinement.thy
@@ -1,50 +1,19 @@
 theory BFS_Refinement
   imports BFS_2 BFS_Subprocedures  Directed_Set_Graphs.Pair_Graph_Imperative
+"HOL-Imperative_HOL.Imperative_HOL" "HOL-Library.IArray"
 begin
 
 record ('imp_dag, 'imp_vis, 'imp_cf) BFS_state_imp =
      parents:: "'imp_dag" current:: "'imp_cf" visited:: "'imp_vis"
 
-
-locale BFS_Imperative = BFS
-  where expand_tree = expand_tree and insert = insert
-  for expand_tree::"'adjmap \<Rightarrow> 'vset \<Rightarrow> 'vset \<Rightarrow> 'adjmap"
-  and insert :: "'ver \<Rightarrow> 'vset \<Rightarrow> 'vset" +
+locale BFS_Imperative_spec = 
 fixes imp_dag_empty::"'imp_dag Heap"
-and imp_dag_assn::"'adjmap \<Rightarrow> 'imp_dag \<Rightarrow> assn"
-and G_imp::"'imp_G"
-and graph_assn::"'adjmap \<Rightarrow> 'imp_G \<Rightarrow> assn"
 and imp_vis_empty::"'imp_vis Heap"
-and imp_vis_assn::"'vset \<Rightarrow> 'imp_vis \<Rightarrow> assn"
-(*and src_imp::"'imp_src Heap"*)
-and imp_src_assn::"'vset \<Rightarrow> 'imp_src \<Rightarrow> assn"
 and imp_src_to_cf::"'imp_src \<Rightarrow> 'imp_cf Heap"
-and imp_cf_assn::"'vset \<Rightarrow> 'imp_cf \<Rightarrow> assn"
 and set_cf_visited::"'imp_vis \<Rightarrow> 'imp_cf \<Rightarrow> 'imp_vis Heap"
 and imp_expand_tree::"'imp_dag \<Rightarrow> 'imp_cf \<Rightarrow> 'imp_vis \<Rightarrow> 'imp_dag Heap"
 and imp_next_frontier::"'imp_cf \<Rightarrow> 'imp_vis \<Rightarrow> 'imp_cf Heap"
 and imp_cf_is_empty::"'imp_cf \<Rightarrow> bool Heap"
-assumes imp_dag_empty: "<emp> imp_dag_empty <imp_dag_assn \<emptyset>\<^sub>G>"
-and imp_vis_empty: "<emp> imp_vis_empty <imp_vis_assn \<emptyset>\<^sub>N>"
-and imp_sf_is_empty: "\<And> S Si. <imp_cf_assn S Si> imp_cf_is_empty Si 
-                       <\<lambda> b. imp_cf_assn S Si * \<up>(b \<longleftrightarrow> S = \<emptyset>\<^sub>N)>"
-and imp_src_to_cf: "\<And> S Si. <imp_src_assn S Si> imp_src_to_cf Si 
-                      <\<lambda> r. imp_src_assn S Si * imp_cf_assn S r>"
-and set_cf_visited: 
-  "\<And> vis imp_vis cf imp_cf. 
-    <imp_vis_assn vis imp_vis * imp_cf_assn cf imp_cf * graph_assn G G_imp>
-    set_cf_visited imp_vis imp_cf
-    <\<lambda> r. imp_vis_assn (vis \<union>\<^sub>G cf) r * imp_cf_assn cf imp_cf * graph_assn G G_imp>"
-and imp_expand_tree:
-  "\<And> dag imp_dag cf imp_cf vis imp_vis.
-    <imp_dag_assn dag imp_dag * imp_cf_assn cf imp_cf * imp_vis_assn vis imp_vis>
-    imp_expand_tree imp_dag imp_cf imp_vis
-    <\<lambda> r. imp_dag_assn (expand_tree dag cf vis) r* imp_cf_assn cf imp_cf 
-              * imp_vis_assn vis imp_vis * graph_assn G G_imp>"
-and imp_next_frontier:  "\<And> cf imp_cf vis imp_vis.
-    <imp_cf_assn cf imp_cf * imp_vis_assn vis imp_vis>
-    imp_next_frontier imp_cf imp_vis
-    <\<lambda> r. imp_cf_assn (next_frontier cf vis) r * imp_vis_assn vis imp_vis * graph_assn G G_imp>"
 begin
 
 partial_function (heap) BFS_imp::
@@ -57,6 +26,51 @@ partial_function (heap) BFS_imp::
                 parents' \<leftarrow> imp_expand_tree (parents state) (current state) visited';
                 current' \<leftarrow> imp_next_frontier (current state) visited';
                 BFS_imp (state \<lparr>parents := parents', visited := visited', current := current' \<rparr> )}}"
+
+definition "initial_state_imp src_imp=  
+  do {cf \<leftarrow> imp_src_to_cf src_imp;
+      p \<leftarrow> imp_dag_empty;
+      v \<leftarrow> imp_vis_empty;
+        return \<lparr>parents = p, current = cf, visited = v\<rparr>}"
+end
+
+locale BFS_Imperative = 
+ BFS  where expand_tree = expand_tree and insert = insert +
+ BFS_Imperative_spec where  imp_src_to_cf = imp_src_to_cf and imp_expand_tree = imp_expand_tree
+ for  imp_src_to_cf :: "'imp_src \<Rightarrow> 'imp_cf Heap"
+  and expand_tree::"'adjmap \<Rightarrow> 'vset \<Rightarrow> 'vset \<Rightarrow> 'adjmap"
+  and insert :: "'ver \<Rightarrow> 'vset \<Rightarrow> 'vset" 
+  and imp_expand_tree::"'imp_dag \<Rightarrow> 'imp_cf \<Rightarrow> 'imp_vis \<Rightarrow> 'imp_dag Heap"+
+
+fixes  G_imp::"'imp_G"
+ and graph_assn::"'adjmap \<Rightarrow> 'imp_G \<Rightarrow> assn"
+ and imp_src_assn::"'vset \<Rightarrow> 'imp_src \<Rightarrow> assn"
+ and imp_dag_assn::"'adjmap \<Rightarrow> 'imp_dag \<Rightarrow> assn"
+ and imp_cf_assn::"'vset \<Rightarrow> 'imp_cf \<Rightarrow> assn"
+ and imp_vis_assn::"'vset \<Rightarrow> 'imp_vis \<Rightarrow> assn"
+assumes imp_dag_empty: "<emp> imp_dag_empty <imp_dag_assn \<emptyset>\<^sub>G>"
+ and imp_vis_empty: "<emp> imp_vis_empty <imp_vis_assn \<emptyset>\<^sub>N>"
+ and imp_sf_is_empty: "\<And> S Si. <imp_cf_assn S Si> imp_cf_is_empty Si 
+                       <\<lambda> b. imp_cf_assn S Si * \<up>(b \<longleftrightarrow> S = \<emptyset>\<^sub>N)>"
+ and imp_src_to_cf: "\<And> S Si. <imp_src_assn S Si> imp_src_to_cf Si 
+                      <\<lambda> r. imp_src_assn S Si * imp_cf_assn S r>"
+ and set_cf_visited: 
+  "\<And> vis imp_vis cf imp_cf. 
+    <imp_vis_assn vis imp_vis * imp_cf_assn cf imp_cf>
+    set_cf_visited imp_vis imp_cf
+    <\<lambda> r. imp_vis_assn (vis \<union>\<^sub>G cf) r * imp_cf_assn cf imp_cf>"
+ and imp_expand_tree:
+  "\<And> dag imp_dag cf imp_cf vis imp_vis.
+    <imp_dag_assn dag imp_dag * imp_cf_assn cf imp_cf * imp_vis_assn vis imp_vis * graph_assn G G_imp>
+    imp_expand_tree imp_dag imp_cf imp_vis
+    <\<lambda> r. imp_dag_assn (expand_tree dag cf vis) r* imp_cf_assn cf imp_cf 
+              * imp_vis_assn vis imp_vis * graph_assn G G_imp>"
+ and imp_next_frontier:  "\<And> cf imp_cf vis imp_vis.
+    <imp_cf_assn cf imp_cf * imp_vis_assn vis imp_vis * graph_assn G G_imp>
+    imp_next_frontier imp_cf imp_vis
+    <\<lambda> r. imp_cf_assn (next_frontier cf vis) r * imp_vis_assn vis imp_vis * graph_assn G G_imp
+          * imp_cf_assn cf imp_cf>"
+begin
 
 definition "state_assn (s::('adjmap, 'vset) BFS_state)
     (imp_s::('imp_dag, 'imp_vis, 'imp_cf) BFS_state_imp) = 
@@ -140,13 +154,6 @@ next
     done     
 qed
 
-
-definition "initial_state_imp src_imp=  
-  do {cf \<leftarrow> imp_src_to_cf src_imp;
-      p \<leftarrow> imp_dag_empty;
-      v \<leftarrow> imp_vis_empty;
-        return \<lparr>parents = p, current = cf, visited = v\<rparr>}"
-
 lemma initial_refine:
  "<imp_src_assn srcs srcs_imp>
   initial_state_imp srcs_imp
@@ -176,4 +183,1091 @@ lemma BFS_program_behaviour:
  
 end
 
+locale imp_2d_array =
+   outer_lookup: imp_map_lookup where lookup = lookup1 and is_map = is_map1+
+   inner_lookup: imp_map_lookup where lookup = lookup2 and is_map = is_map2+
+   outer_empty: imp_map_empty where empty = empty1 and is_map = is_map1 +
+   inner_empty: imp_map_empty where empty = empty2 and is_map = is_map2+
+   outer_upd: imp_map_update where is_map = is_map1 and update = update1+
+   inner_upd: imp_map_update where is_map = is_map2 and update = update2
+ for lookup1 :: "nat \<Rightarrow> 'outer \<Rightarrow> 'inner option Heap"
+   and lookup2 :: "nat \<Rightarrow> 'inner \<Rightarrow> 'val option Heap"
+   and is_map1 and is_map2 and empty1::"'outer Heap" and empty2::"'inner Heap"
+   and update1 and update2
+begin
+
+definition lookup_2d :: "'outer \<Rightarrow> nat \<Rightarrow> nat \<Rightarrow> 'val option Heap" where
+  "lookup_2d M i j = do {
+    opt_row \<leftarrow> lookup1 i M;
+    (case opt_row of
+      None \<Rightarrow> return None
+    | Some row_map \<Rightarrow> do {
+        val \<leftarrow> lookup2 j row_map;
+        return val
+      })
+  }"
+
+definition update_2d :: "nat \<Rightarrow> nat \<Rightarrow> 'val \<Rightarrow> 'outer \<Rightarrow> 'outer Heap" where
+  "update_2d i j v M = do {
+    opt_row \<leftarrow> lookup1 i M;
+    row_map \<leftarrow> (case opt_row of
+                 None \<Rightarrow> empty2   
+               | Some rm \<Rightarrow> return rm); 
+    row_map' \<leftarrow> update2 j v row_map;
+    M' \<leftarrow> update1 i row_map' M; 
+    return M'
+  }"
+
+definition 
+"prog v = do {
+  empt \<leftarrow> empty1;
+  arr2 \<leftarrow> update_2d 0 0 v  empt;
+  val \<leftarrow> lookup_2d arr2 0 0;
+  return val
+}"
+
+lemma "<emp> prog v <\<lambda> r. \<up> (r = Some v)>"
+  unfolding prog_def update_2d_def lookup_2d_def
+  apply auto
+  by sep_auto
+
+lemma "<emp> prog v <\<lambda> r. \<up> (r = Some v) *  true>"
+  unfolding prog_def update_2d_def lookup_2d_def
+  apply auto
+  by sep_auto
+
 end
+
+setup Locale_Code.open_block 
+interpretation matr: imp_2d_array iam_lookup iam_lookup
+   is_iam is_iam iam_new iam_new iam_update iam_update
+by unfold_locales
+setup Locale_Code.close_block 
+print_theorems
+
+definition "iam_2dim_update = 
+(matr.update_2d::(nat \<Rightarrow> nat \<Rightarrow> nat 
+\<Rightarrow> nat option array option array \<Rightarrow> nat option array option array Heap))"
+definition "iam_2dim_lookup =
+( matr.lookup_2d::(nat option array option array \<Rightarrow> nat \<Rightarrow> nat \<Rightarrow> nat option Heap))"
+definition "iam_2dim_empty = (iam_new::nat option array option array Heap)"
+definition "prog = (matr.prog::(nat \<Rightarrow> nat option Heap))"
+
+export_code iam_2dim_update iam_2dim_lookup iam_2dim_empty nat_of_integer prog checking SML_imp
+
+ML \<open>val prog = @{code prog}
+    val noi = @{code nat_of_integer} 
+    val final = prog (noi 1) ()\<close>
+
+ML \<open>
+   val iam_2dim_empty = @{code iam_2dim_empty} ()
+   val iam_2dim_lookup = @{code iam_2dim_lookup}
+   val iam_2dim_update = @{code iam_2dim_update}
+   val noi = @{code nat_of_integer}
+   val _ = iam_2dim_update (noi 1) (noi 1) (noi 10) iam_2dim_empty ()
+   val _ = iam_2dim_update (noi 2) (noi 1) (noi 33) iam_2dim_empty ()
+   val array_at_1_1 = iam_2dim_lookup iam_2dim_empty (noi 1) (noi 1) ()
+   val array_at_2_1 = iam_2dim_lookup iam_2dim_empty (noi 2) (noi 1) ()
+   \<close>
+
+lemma "i \<in> set xs \<Longrightarrow> foldr (\<lambda> i as. assn (f i) (g i) * as) xs emp \<Longrightarrow>\<^sub>A assn (f i) (g i) * true"
+  apply(induction xs)
+   apply auto
+   apply sep_auto
+  using ent_true_drop(1) star_aci(2) by fastforce
+
+lemma assn_over_finite_extract_one:
+     "\<lbrakk>finite S; i \<in> S\<rbrakk> \<Longrightarrow> Finite_Set.fold (\<lambda> i as. assn (f i) (g i) * as) emp S
+           = assn (f i) (g i) * Finite_Set.fold (\<lambda> i as. assn (f i) (g i) * as) emp (S - {i})"
+  apply(induction rule: finite_induct)
+  subgoal
+    by simp
+  apply(subst comp_fun_commute_on.fold_insert_remove[where S = UNIV])
+  subgoal
+    by(auto intro!: comp_fun_commute_on.intro ext simp add: star_aci(3))
+  subgoal
+    by simp
+  subgoal
+    by simp
+  subgoal for x F
+    apply(cases "i = x")
+    subgoal
+      by auto
+    subgoal
+      apply(subst insert_minus_eq)
+       apply simp
+      apply(subst comp_fun_commute_on.fold_insert_remove[where S = UNIV])
+      subgoal
+        by(auto intro!: comp_fun_commute_on.intro ext simp add: star_aci(3))
+      subgoal by simp
+      subgoal by simp
+      apply auto
+      apply sep_auto
+      by (smt (verit, del_insts) assn_aci(11) fr_refl star_aci(2))
+    done
+  done
+
+lemma assn_take_one_from_dom: 
+  "\<up> (finite (dom S)) * \<up> (S i = Some x) * Finite_Set.fold (\<lambda> i as. assn (f i) (g i) * as) emp (dom S)
+ = \<up> (finite (dom S)) *  \<up> (S i = Some x) *
+          assn (f i) (g i) * Finite_Set.fold (\<lambda> i as. assn (f i) (g i) * as) emp (dom S - {i})"
+  apply(rule ent_iffI)
+  by(sep_auto | subst assn_over_finite_extract_one[of "dom S" i] | force)+
+  
+lemma assn_over_finite_insert_one:
+     "\<lbrakk>finite S; i \<notin> S\<rbrakk> \<Longrightarrow> Finite_Set.fold (\<lambda> i as. assn (f i) (g i) * as) emp (Set.insert i S)
+           = assn (f i) (g i) * Finite_Set.fold (\<lambda> i as. assn (f i) (g i) * as) emp S"
+  by(simp add: assn_over_finite_extract_one[of "Set.insert i S" i, simplified])
+
+lemma assns_over_set_cong:
+  "\<lbrakk>finite S; \<And> i. i \<in> S \<Longrightarrow> assn (f i) (g i) = assn' (f' i) (g' i)\<rbrakk> \<Longrightarrow>
+     Finite_Set.fold (\<lambda> i as. assn (f i) (g i) * as) emp S = 
+     Finite_Set.fold (\<lambda> i as. assn' (f' i) (g' i) * as) emp S"
+  apply(rule Finite_Set.fold_cong[where S = UNIV])
+  using star_aci(3) by (auto intro!: comp_fun_commute_on.intro)
+
+lemma pure_assn_over_finite_set:
+   "finite S \<Longrightarrow> Finite_Set.fold (\<lambda> i as. \<up> (P i) * as) emp S = \<up> (\<forall> i \<in> S. P i)"
+  by(induction rule: finite_induct)
+    (simp add: assn_over_finite_insert_one[where assn = "\<lambda> i j. \<up> (P i)" and f = id, simplified])+
+
+context
+  imp_2d_array
+begin
+
+definition is_2d_map :: "(nat \<Rightarrow> nat \<Rightarrow> 'val option) \<Rightarrow> 'outer \<Rightarrow> assn" where
+  "is_2d_map f M = (\<exists>\<^sub>A A . 
+      is_map1 A M * \<up> (finite (dom A)) *  \<up> (\<forall> i j. A i = None \<longrightarrow> f i j = None)*
+       Finite_Set.fold (\<lambda> i ass. is_map2 (f i) (the (A i)) * ass) emp (dom A))"
+
+definition is_2d_map' :: "(nat \<Rightarrow> nat \<Rightarrow> 'val option) \<Rightarrow> 'outer \<Rightarrow> (nat \<Rightarrow> 'inner option) \<Rightarrow> assn" where
+  "is_2d_map' f M A = ( 
+      is_map1 A M * \<up> (finite (dom A)) *  \<up> (\<forall> i j. A i = None \<longrightarrow> f i j = None)*
+       Finite_Set.fold (\<lambda> i ass. is_map2 (f i) (the (A i)) * ass) emp (dom A))"
+
+
+lemma forw_subst_assn:
+  "x = y \<Longrightarrow> P x \<Longrightarrow>\<^sub>A Q x \<Longrightarrow> P x \<Longrightarrow>\<^sub>A Q y"
+  by sep_auto
+
+lemma impl_of_exes_assn:"(\<And> x. P x \<Longrightarrow>\<^sub>A Q x) \<Longrightarrow> \<exists>\<^sub>A x. P x \<Longrightarrow>\<^sub>A \<exists>\<^sub>A x. Q x"
+  apply(rule ent_ex_preI)
+  apply(rule ent_ex_postI)
+  by auto
+
+lemma same_assn: "A = B \<Longrightarrow> A \<Longrightarrow>\<^sub>A B" for A B
+  by simp
+
+lemma update_2d_rule:
+ "<is_2d_map M Mi>
+  update_2d i j v Mi
+  <\<lambda> Mi. is_2d_map (\<lambda> x y. if x = i \<and> y= j then Some v else M x y) Mi >"
+  unfolding update_2d_def is_2d_map_def
+  apply(rule ht_bind[where R =
+        "\<lambda> r. \<exists>\<^sub>AA. is_map1 A Mi * \<up> (finite (dom A)) * \<up> (\<forall>i j. A i = None \<longrightarrow> M i j = None) *
+           Finite_Set.fold (\<lambda>i. (*) (is_map2 (M i) (the (A i)))) emp (dom A) * \<up> (r = A i)"])
+  subgoal
+    by sep_auto
+  subgoal for or
+    apply(clarsimp split!: option.split)
+    subgoal
+      apply(rule ht_bind[where R =
+            "\<lambda> r. \<exists>\<^sub>AA. is_map1 A Mi * \<up> (finite (dom A)) * \<up> (\<forall>i. A i = None \<longrightarrow> (\<forall>j. M i j = None)) *
+           Finite_Set.fold (\<lambda>i. (*) (is_map2 (M i) (the (A i)))) emp (dom A) *
+           \<up> (A i = None) * is_map2 (\<lambda>x. None) r * \<up> (\<forall>j. M i j = None)"])
+      subgoal
+        by sep_auto
+      subgoal for row_map
+        apply(rule ht_bind[where R =
+          "\<lambda> r. \<exists>\<^sub>AA. is_map1 A Mi * \<up> (finite (dom A)) * \<up> (\<forall>i. A i = None \<longrightarrow> (\<forall>j. M i j = None)) *
+           Finite_Set.fold (\<lambda>i. (*) (is_map2 (M i) (the (A i)))) emp (dom A) *
+           \<up> (A i = None) *is_map2 [j \<mapsto> v] r * \<up> (\<forall>j. M i j = None)"])
+        subgoal
+          by sep_auto
+        subgoal for row_map'
+          apply(rule ht_cons_prec[where P = P and P' = P for P , where Q =
+                "\<lambda> Mi. \<exists>\<^sub>AA. is_map1 A Mi * \<up> (finite (dom A)) * \<up> (\<forall>ia ja. A ia = None \<longrightarrow> M ia ja = None) *
+           Finite_Set.fold (\<lambda>i. (*) (is_map2 (M i) (the (A i)))) emp (dom A - {i}) * \<up> (A i = Some row_map') *
+           is_map2 [j \<mapsto> v] row_map' * \<up> (\<forall>j. M i j = None)"])
+          subgoal by sep_auto
+          subgoal for Mi
+            apply(rule ent_ex_preI)
+            subgoal for A
+              apply(rule ent_ex_postI[of _ _ A])
+              apply sep_auto
+              subgoal
+                apply(subst assn_over_finite_extract_one[of "dom A" i])
+                  apply simp
+                 apply force
+                apply simp
+
+                apply sep_auto
+                apply(subst assns_over_set_cong[of "dom A - {i}" is_map2
+                       "\<lambda> ia y. if ia = i \<and> y = j then Some v else M ia y" "\<lambda> ia. the (A ia)"
+                      is_map2 M "\<lambda> ia. the (A ia)"])
+                  apply simp
+                 apply simp
+                apply(rule forw_subst_assn[of "[j \<mapsto> v]" "\<lambda>y. if y = j then Some v else M i y"])
+                subgoal 
+                  by (auto intro!: ext) 
+                by sep_auto
+               by sep_auto
+             done
+          apply sep_auto
+          subgoal for A a b r
+            apply(rule mod_exI[of _ "A(i \<mapsto> row_map')"])
+            apply sep_auto
+            apply(subst (asm) assns_over_set_cong[of "dom A" is_map2 M "\<lambda> i. the (A i)" is_map2 M
+ "\<lambda> ia. the (if ia = i then Some row_map' else A ia)"])
+              apply simp
+             apply force
+            apply(subst set_minus_singleton_eq)
+             apply force
+            by simp
+          done
+        done
+      done
+    subgoal for opt_row
+      apply(rule ht_cons_prec[where P' = "\<exists>\<^sub>AA. is_map1 A Mi * \<up> (finite (dom A)) * \<up> (\<forall>i. A i = None \<longrightarrow> (\<forall>j. M i j = None)) *
+          Finite_Set.fold (\<lambda>i. (*) (is_map2 (M i) (the (A i)))) emp (dom A - {i}) *
+          \<up> (A i = Some opt_row) * is_map2 (M i) (the (A i))", where Q = Q and Q' = Q for Q ])
+      subgoal
+        apply(rule impl_of_exes_assn)
+        subgoal for A
+          apply sep_auto
+          subgoal
+            apply(subst assn_over_finite_extract_one[of "dom A" i is_map2 M "\<lambda> i. the (A i)"])
+              apply simp
+             apply (metis domI)
+            by sep_auto
+          using mod_pure_star_dist by auto
+        done
+      subgoal by sep_auto
+      apply(rule ht_bind[where R = "\<lambda> r. \<exists>\<^sub>AA. is_map1 A Mi * \<up> (finite (dom A)) * \<up> (\<forall>i. A i = None \<longrightarrow> (\<forall>j. M i j = None)) *
+           Finite_Set.fold (\<lambda>i. (*) (is_map2 (M i) (the (A i)))) emp (dom A - {i}) *
+           \<up> (A i = Some opt_row) *
+           is_map2 ((M i)(j \<mapsto> v)) r"])
+      subgoal
+        by sep_auto
+      subgoal for opt_row'
+        apply(rule ht_cons_prec[where P = P and P' = P for P, where Q =
+                "\<lambda> r. \<exists>\<^sub>AA. is_map1 (A(i \<mapsto> opt_row')) r * \<up> (finite (dom A)) * \<up> (\<forall>i. A i = None \<longrightarrow> (\<forall>j. M i j = None)) *
+           Finite_Set.fold (\<lambda>i. (*) (is_map2 (M i) (the (A i)))) emp (dom A - {i}) *
+           \<up> (A i = Some opt_row) *
+           is_map2 ((M i)(j \<mapsto> v)) opt_row'"])
+      subgoal by sep_auto
+       defer
+      subgoal
+        by sep_auto
+      subgoal for Mi'
+        apply(rule ent_ex_preI)
+        subgoal for A
+          apply(rule ent_ex_postI[of _ _ "A(i \<mapsto> opt_row')"])
+          apply (sep_auto simp: mod_pure_star_dist)
+          apply(rule same_assn)
+          apply(subst semigroup_mult_class.mult.assoc)
+          apply(rule arg_cong2[where f = "(*)"])
+           apply simp
+          apply(subst insert_absorb[of i "dom A"])
+           apply force
+          apply(subst assn_over_finite_extract_one[of "dom A" i])
+            apply simp
+           apply force
+          apply(subst ab_semigroup_mult_class.mult.commute)
+          apply(rule arg_cong2[where f = "(*)"])
+          subgoal
+            apply sep_auto
+            by(auto intro!: arg_cong2[where f = is_map2])
+          by(auto intro!: assns_over_set_cong arg_cong2[where f = is_map2])
+        done
+      done
+    done
+  done
+  done
+
+lemma empty_2d_rule:
+  "<emp> empty1 <\<lambda> r. is_2d_map (\<lambda> x y. None) r>"
+  unfolding is_2d_map_def
+  using outer_empty.empty_rule
+  by (sep_auto intro: mod_exI[of _ "\<lambda> x. None"])
+
+definition 
+"prog' v v' v''= do {
+  arr \<leftarrow> empty1;
+  arr \<leftarrow> update_2d 0 0 v arr;
+  arr \<leftarrow> update_2d 0 1 v' arr;
+  arr \<leftarrow> update_2d 4 1 v'' arr;
+  arr \<leftarrow> update_2d 4 6 v'' arr;
+  val \<leftarrow> lookup_2d arr 4 1;
+  val' \<leftarrow> lookup_2d arr 0 10;
+  case val of Some val \<Rightarrow> do 
+        {
+        case val' of Some val' \<Rightarrow> return (val = val') |
+           None \<Rightarrow> return False
+        }
+  | None \<Rightarrow> return False
+}"
+
+(*
+lemma loop_fst_d_rule:
+"<is_2d_map M Mi>
+ lookup1 i Mi
+<\<lambda> r. is_2d_map M Mi \<and>\<^sub>A is_map2 (M i) r>"
+  apply(auto simp add: is_2d_map_def)
+  using outer_lookup.lookup_rule apply sep_auto
+  subgoal for A a b
+    apply(rule mod_exI[of _ A])
+    using outer_lookup.lookup_rule[of A Mi i] apply sep_auto
+
+lemma "is_2d_map' f M A \<Longrightarrow>\<^sub>A is_map2 (f i) (the (A i)) *  true"
+  sorry
+
+lemma loop_fst_d_rule:
+"<is_map1 M Mi>
+ lookup1 i Mi
+<\<lambda> r. is_map1 M Mi * \<up> (r = M i)>"
+  sorry
+*)
+lemma lookup_2d_rule:
+ "<is_2d_map M Mi>
+  lookup_2d Mi i j
+  <\<lambda> r. is_2d_map M Mi * \<up> (r = M i j)>"
+  unfolding lookup_2d_def is_2d_map_def
+  apply(rule ht_bind[where R =
+     "\<lambda> r. \<exists>\<^sub>AA. is_map1 A Mi * \<up> (finite (dom A)) * \<up> (\<forall>i j. A i = None \<longrightarrow> M i j = None) *
+           Finite_Set.fold (\<lambda>i. (*) (is_map2 (M i) (the (A i)))) emp (dom A) * \<up> (r = A i)"])
+  subgoal
+    by sep_auto
+  subgoal for mm
+    apply(clarsimp split!: option.split)
+    subgoal
+      using ht_frame
+      using outer_lookup.lookup_rule  
+      by sep_auto 
+    subgoal for m
+      apply(rule ht_cons_prec[where P'=
+       "\<exists>\<^sub>AA. is_map1 A Mi * \<up> (finite (dom A)) * \<up> (\<forall>i. A i = None \<longrightarrow> (\<forall>j. M i j = None)) *
+          Finite_Set.fold (\<lambda>i. (*) (is_map2 (M i) (the (A i)))) emp (dom A - {i}) *
+          \<up> (Some m = A i) * is_map2 (M i) m"
+      and Q = "\<lambda> x. \<exists>\<^sub>AA. is_map1 A Mi * \<up> (finite (dom A)) * \<up> (\<forall>i. A i = None \<longrightarrow> (\<forall>j. M i j = None)) *
+          Finite_Set.fold (\<lambda>i. (*) (is_map2 (M i) (the (A i)))) emp (dom A - {i}) *
+          \<up> (Some m = A i) * is_map2 (M i) m *\<up> (x = M i j)"])
+      subgoal
+        apply sep_auto
+        apply(rule ent_ex_preI)
+        subgoal for A
+          apply sep_auto
+          apply(subst assn_over_finite_extract_one[of "dom A" i])
+            apply simp
+          subgoal
+            apply auto
+            by metis
+          apply(rule ent_ex_postI[of _ _ A])
+          apply sep_auto
+          by (metis (no_types, lifting) assn_aci(11) ent_refl option.sel)
+        done
+      subgoal for r
+        apply sep_auto
+        apply(rule ent_ex_preI)
+        subgoal for A
+          apply(rule ent_ex_postI[of _ _ A])
+          apply sep_auto
+          apply(subst assn_over_finite_extract_one[of "dom A" i])
+            apply simp
+          subgoal
+            apply auto
+            by metis
+          subgoal
+            apply sep_auto
+            by (metis (no_types, lifting) assn_aci(11) ent_refl option.sel)
+          by sep_auto
+        done
+      by sep_auto
+    done
+  done
+(*
+lemma lookup_2d_rule':
+ "<is_2d_map' M Mi A>
+  lookup_2d Mi i j
+  <\<lambda> r. is_2d_map' M Mi A* \<up> (r = M i j)>"
+  unfolding lookup_2d_def is_2d_map'_def
+  apply(rule ht_bind[where R =
+     "\<lambda> r. is_map1 A Mi * \<up> (finite (dom A)) * \<up> (\<forall>i j. A i = None \<longrightarrow> M i j = None) *
+           Finite_Set.fold (\<lambda>i. ( * ) (is_map2 (M i) (the (A i)))) emp (dom A) * \<up> (r = A i)"])
+  subgoal
+    by sep_auto
+  subgoal for mm
+    apply(clarsimp split!: option.split)
+    subgoal
+      using ht_frame
+      using outer_lookup.lookup_rule  
+      by sep_auto 
+    subgoal for m
+      apply(rule ht_cons_prec[where P'=
+       "is_map1 A Mi * \<up> (finite (dom A)) * \<up> (\<forall>i. A i = None \<longrightarrow> (\<forall>j. M i j = None)) *
+          Finite_Set.fold (\<lambda>i. ( * ) (is_map2 (M i) (the (A i)))) emp (dom A - {i}) *
+          \<up> (Some m = A i) * is_map2 (M i) m"
+      and Q = "\<lambda> x. is_map1 A Mi * \<up> (finite (dom A)) * \<up> (\<forall>i. A i = None \<longrightarrow> (\<forall>j. M i j = None)) *
+          Finite_Set.fold (\<lambda>i. ( * ) (is_map2 (M i) (the (A i)))) emp (dom A - {i}) *
+          \<up> (Some m = A i) * is_map2 (M i) m *\<up> (x = M i j)"])
+      subgoal
+        apply sep_auto
+          apply(subst assn_over_finite_extract_one[of "dom A" i])
+            apply simp
+          subgoal
+            apply auto
+            by metis
+             apply sep_auto
+             apply (metis (no_types, lifting) assn_aci(11) ent_refl option.sel)
+          by sep_auto
+      subgoal for r
+        apply sep_auto
+          apply(subst assn_over_finite_extract_one[of "dom A" i])
+            apply simp
+          subgoal
+            apply auto
+            by metis
+          subgoal
+            apply sep_auto
+            by (metis (no_types, lifting) assn_aci(11) ent_refl option.sel)
+          by sep_auto
+      by sep_auto
+    done
+  done*)
+(*
+lemma lookup_2d_rule:
+ "<is_2d_map M Mi>
+  lookup_2d Mi i j
+  <\<lambda> r. is_2d_map M Mi * \<up> (r = M i j)>"
+  unfolding lookup_2d_def is_2d_map_def
+  apply(rule ht_bind[where R =
+     "\<lambda> r. is_2d_map M Mi * \<up> (return r = lookup1 i Mi)"])
+  subgoal
+    unfolding is_2d_map_def
+    apply sep_auto
+    subgoal for A a b
+
+
+
+  subgoal for mm
+    apply(clarsimp split!: option.split)
+    subgoal
+      by sep_auto 
+    subgoal for m
+      apply(rule ht_cons_prec[where P'=
+       "\<exists>\<^sub>AA. is_map1 A Mi * \<up> (finite (dom A)) * \<up> (\<forall>i. A i = None \<longrightarrow> (\<forall>j. M i j = None)) *
+          Finite_Set.fold (\<lambda>i. ( * ) (is_map2 (M i) (the (A i)))) emp (dom A - {i}) *
+          \<up> (Some m = A i) * is_map2 (M i) m"
+      and Q = "\<lambda> x. \<exists>\<^sub>AA. is_map1 A Mi * \<up> (finite (dom A)) * \<up> (\<forall>i. A i = None \<longrightarrow> (\<forall>j. M i j = None)) *
+          Finite_Set.fold (\<lambda>i. ( * ) (is_map2 (M i) (the (A i)))) emp (dom A - {i}) *
+          \<up> (Some m = A i) * is_map2 (M i) m *\<up> (x = M i j)"])
+      subgoal
+        apply sep_auto
+        apply(rule ent_ex_preI)
+        subgoal for A
+          apply sep_auto
+          apply(subst assn_over_finite_extract_one[of "dom A" i])
+            apply simp
+          subgoal
+            apply auto
+            by metis
+          apply(rule ent_ex_postI[of _ _ A])
+          apply sep_auto
+          by (metis (no_types, lifting) assn_aci(11) ent_refl option.sel)
+        done
+      subgoal for r
+        apply sep_auto
+        apply(rule ent_ex_preI)
+        subgoal for A
+          apply(rule ent_ex_postI[of _ _ A])
+          apply sep_auto
+          apply(subst assn_over_finite_extract_one[of "dom A" i])
+            apply simp
+          subgoal
+            apply auto
+            by metis
+          subgoal
+            apply sep_auto
+            by (metis (no_types, lifting) assn_aci(11) ent_refl option.sel)
+          by sep_auto
+        done
+      by sep_auto
+    done
+  done
+*)
+
+lemma "<emp> prog' v v' v''<\<lambda> r. \<up> (\<not> r)>"
+  using update_2d_rule lookup_2d_rule empty_2d_rule
+  unfolding prog'_def 
+  by sep_auto
+
+end
+
+locale BFS_subprocedures_Imperative_spec =
+fixes unvisited_neighbs::"'nh \<Rightarrow> 'vis \<Rightarrow> 'nh_nv Heap"
+and add_to_working_frontier::"'wfront \<Rightarrow> 'nh_nv \<Rightarrow> 'wfront Heap"
+and to_ordinary_frontier::"'wfront \<Rightarrow> 'front Heap"
+and frontier_fold_imp::"('ver \<Rightarrow> 'wfront \<Rightarrow> 'wfront Heap) \<Rightarrow> 'front \<Rightarrow> 'wfront \<Rightarrow> 'wfront Heap"
+and lookup_imp :: "'ver \<Rightarrow> 'adjmap_imp \<Rightarrow> 'nh option Heap"
+and nh_emp::"'nh Heap"
+and wf_empty::"'wfront Heap"
+and add_to_dag_nh::"'nh_ex \<Rightarrow> 'nh_nv \<Rightarrow> 'nh_ex Heap"
+and update_dag_imp::"'ver \<Rightarrow> 'nh_ex \<Rightarrow> 'dag \<Rightarrow> 'dag Heap"
+and to_dag_nh::"'nh_nv \<Rightarrow> 'nh_ex Heap"
+and lookup_dag_imp::"'ver \<Rightarrow> 'dag \<Rightarrow> 'nh_ex option Heap"
+and is_neighb_nv_emp::"'nh_nv \<Rightarrow> bool Heap"
+and dag_fold_imp::"('ver \<Rightarrow> 'dag \<Rightarrow> 'dag Heap) \<Rightarrow> 'front \<Rightarrow> 'dag \<Rightarrow> 'dag Heap"
+begin
+
+definition "neighbourhood_imp Gi v = 
+  do {nhd \<leftarrow> lookup_imp v Gi;
+      case nhd of None \<Rightarrow> nh_emp
+      | Some nhd \<Rightarrow> return nhd}"
+
+definition "next_frontier_body Gi vis u nf = 
+   do {nhd \<leftarrow> neighbourhood_imp Gi u;
+       uv_nhd \<leftarrow> unvisited_neighbs nhd vis;
+       add_to_working_frontier nf uv_nhd}"
+
+definition "next_frontier_imperative Gi frontier vis =
+    do {nf \<leftarrow> wf_empty;
+        nf' \<leftarrow> frontier_fold_imp (next_frontier_body Gi vis) frontier nf;
+        to_ordinary_frontier nf'}"
+
+definition "add_dag_neighbs_imp Gi u more_nh = 
+ do {is_emp \<leftarrow> is_neighb_nv_emp more_nh;
+   if is_emp then return Gi
+   else
+   do { nho \<leftarrow> lookup_dag_imp u Gi;
+      case nho of None \<Rightarrow>
+        do { nho \<leftarrow> to_dag_nh more_nh;
+             update_dag_imp u nho Gi
+            }
+     | Some nho \<Rightarrow>
+      do {nho \<leftarrow> add_to_dag_nh nho more_nh;
+          update_dag_imp u nho Gi }
+    }
+  }"
+
+definition "expand_tree_body Gi vis u dag = 
+   do {nhd \<leftarrow> neighbourhood_imp Gi u;
+       uv_nhd \<leftarrow> unvisited_neighbs nhd vis;
+       add_dag_neighbs_imp dag u uv_nhd}"
+
+definition "expand_tree_imp Gi dag front vis = dag_fold_imp (expand_tree_body Gi vis) front dag"
+
+end
+
+term foldM
+
+lemma ht_exPI:"<P> c <\<lambda> r. Q x r> \<Longrightarrow> <P> c <\<lambda> r. \<exists>\<^sub>A x. Q x r>"
+  by sep_auto
+
+lemma ht_ex_pre_and_post_I:"(\<And> x. <P x> c <\<lambda> r. Q x r>) \<Longrightarrow> <\<exists>\<^sub>A x. P x> c <\<lambda> r. \<exists>\<^sub>A x. Q x r>"
+  by sep_auto
+
+lemma ht_ex_with_change_pre_and_post_I: 
+  "(\<And> x. <P x> c <\<lambda> r. Q (f x) r>) \<Longrightarrow> <\<exists>\<^sub>A x. P x> c <\<lambda> r. \<exists>\<^sub>A x. Q x r>"
+  by sep_auto
+
+locale BFS_subprocedures_Imperative =
+
+BFS_subprocedures where fold_vset = fold_vset and fold_adjmap = fold_adjmap +
+imp_map_empty is_dag dag_empty +
+BFS_subprocedures_Imperative_spec where unvisited_neighbs= unvisited_neighbs and
+  add_to_working_frontier = add_to_working_frontier and
+  to_ordinary_frontier = to_ordinary_frontier and 
+  frontier_fold_imp = frontier_fold_imp and
+  lookup_imp = lookup_imp and 
+  nh_emp = nh_emp and
+  wf_empty = wf_empty and
+  add_to_dag_nh = add_to_dag_nh and
+  update_dag_imp = update_dag_imp and
+  to_dag_nh = to_dag_nh and
+  lookup_dag_imp = lookup_dag_imp and
+  is_neighb_nv_emp = is_neighb_nv_emp and
+  dag_fold_imp = dag_fold_imp+
+imp_graph_map: imp_map_lookup is_map lookup_imp +
+imp_dag_map: imp_map_lookup is_dag lookup_dag_imp +
+imp_dag_map_upd: imp_map_update is_dag update_dag_imp 
+for  fold_vset::"('ver \<Rightarrow> 'vset \<Rightarrow> 'vset) \<Rightarrow> 'vset \<Rightarrow> 'vset \<Rightarrow> 'vset"
+and fold_adjmap::"('ver \<Rightarrow> 'adjmap \<Rightarrow> 'adjmap) \<Rightarrow> 'vset \<Rightarrow> 'adjmap \<Rightarrow> 'adjmap"
+and unvisited_neighbs::"'nh \<Rightarrow> 'vis \<Rightarrow> 'nh_nv Heap"
+and add_to_working_frontier::"'wfront \<Rightarrow> 'nh_nv \<Rightarrow> 'wfront Heap"
+and to_ordinary_frontier::"'wfront \<Rightarrow> 'front Heap"
+and frontier_fold_imp::"('ver \<Rightarrow> 'wfront \<Rightarrow> 'wfront Heap) \<Rightarrow> 'front \<Rightarrow> 'wfront \<Rightarrow> 'wfront Heap"
+and lookup_imp :: "'ver \<Rightarrow> 'adjmap_imp \<Rightarrow> 'nh option Heap"
+and nh_emp::"'nh Heap"
+and wf_empty::"'wfront Heap"
+and is_map 
+and is_dag
+and lookup_dag_imp::"'ver \<Rightarrow> 'dag \<Rightarrow> 'nh_ex option Heap"
+and update_dag_imp
+and add_to_dag_nh::"'nh_ex \<Rightarrow> 'nh_nv \<Rightarrow> 'nh_ex Heap"
+and to_dag_nh::"'nh_nv \<Rightarrow> 'nh_ex Heap"
+and is_neighb_nv_emp::"'nh_nv \<Rightarrow> bool Heap"
+and dag_fold_imp::"('ver \<Rightarrow> 'dag \<Rightarrow> 'dag Heap) \<Rightarrow> 'front \<Rightarrow> 'dag \<Rightarrow> 'dag Heap"
+and dag_empty+
+fixes is_neighb::"'vset \<Rightarrow> 'nh \<Rightarrow> assn"
+and is_vis::"'vset \<Rightarrow> 'vis \<Rightarrow> assn"
+and is_neighb_nv::"'vset \<Rightarrow> 'nh_nv \<Rightarrow> assn"
+and is_wfront::"'vset \<Rightarrow> 'wfront \<Rightarrow> assn"
+and is_front::"'vset \<Rightarrow> 'front \<Rightarrow> assn"
+and is_dag_nh::"'vset \<Rightarrow> 'nh_ex \<Rightarrow> assn"
+assumes nd_emp_rule: "<emp> nh_emp <is_neighb \<emptyset>\<^sub>N >"
+and wf_empty_rule: "<emp> wf_empty<is_wfront \<emptyset>\<^sub>N>"
+and is_neighb_nv_emp_rule: 
+  "\<And> nnh nnhi. <is_neighb_nv nnh nnhi> 
+     is_neighb_nv_emp nnhi
+     <\<lambda> r. is_neighb_nv nnh nnhi * \<up> (r \<longleftrightarrow> (nnh = \<emptyset>\<^sub>N))>"
+and is_neighb_nv_invar: "\<And> nnh nnhi. is_neighb_nv nnh nnhi = is_neighb_nv nnh nnhi * \<up> (vset_inv nnh) "
+and unvisited_neighbs_rule: 
+  "\<And> nd ndi vis visi. 
+     <is_neighb nd ndi * is_vis vis visi> 
+         unvisited_neighbs  ndi visi 
+     <\<lambda> r. is_neighb nd ndi * is_vis vis visi * is_neighb_nv (diff nd vis) r>"
+and add_to_working_frontier_rule:
+   "\<And> f fi nh nhi.
+     <is_wfront f fi * is_neighb_nv nh nhi>
+         add_to_working_frontier fi nhi
+     <\<lambda> r. is_wfront (f \<union>\<^sub>G nh) r * is_neighb_nv nh nhi>"
+and frontier_fold_rule:
+   "\<And> front fronti init initi F fi f. 
+      (\<And> u front fronti. 
+          <F * is_wfront front fronti> 
+            fi u fronti 
+          <\<lambda> r. F * is_wfront (f u front) r>) \<Longrightarrow>
+      <F* is_front front fronti * is_wfront init initi> 
+         frontier_fold_imp fi fronti initi 
+      <\<lambda>r. F * is_front front fronti * is_wfront (fold_vset f front init) r>"
+and to_ordinary_frontier_rule:
+  "\<And> f wfi. <is_wfront f wfi> to_ordinary_frontier wfi <\<lambda> r. is_wfront f wfi * is_front f r>"
+and add_to_dag_nh_rule: 
+   "\<And> dag_nh dag_nhi nnh nnhi.
+      <is_dag_nh dag_nh dag_nhi * is_neighb_nv nnh nnhi> 
+         add_to_dag_nh dag_nhi nnhi
+       <\<lambda> r. is_dag_nh (dag_nh \<union>\<^sub>G nnh) r * is_neighb_nv nnh nnhi>"
+and to_dag_nh_rule: 
+   "\<And> nh nhi.
+      <is_neighb_nv nh nhi> 
+         to_dag_nh nhi
+       <\<lambda> dag_nhi. is_dag_nh nh dag_nhi * is_neighb_nv nh nhi>"
+and dag_fold_imp:
+   "\<And> front fronti init initi dag_assn F fi f. 
+      (\<And> dag dagi u.
+        < F * dag_assn dag dagi> fi u dagi  <\<lambda>r. F * dag_assn (f u dag) r>) \<Longrightarrow>
+      < F * is_front front fronti * dag_assn init initi> 
+         dag_fold_imp fi fronti initi 
+      <\<lambda>r. F * is_front front fronti * dag_assn (fold_adjmap f front init) r>"
+begin
+
+definition "graph_assn Gr Gri = 
+  (\<exists>\<^sub>A A. is_map A Gri * \<up> (finite (dom A)) *  \<up> (dom (lookup Gr) = dom A)*
+       Finite_Set.fold (\<lambda> i ass. is_neighb (the (lookup Gr i)) (the (A i)) * ass) emp (dom A))"
+(*
+definition "graph_assn_except Gr Gri v = 
+  (\<exists>\<^sub>A A. is_map A Gri * \<up> (finite (dom A)) *  \<up> (dom (lookup Gr) = dom A)*
+       Finite_Set.fold (\<lambda> i ass. is_neighb (the (lookup Gr i)) (the (A i)) * ass) emp (dom A - {v}))"
+
+
+lemma neighbourhood_imp_rule:
+   "<graph_assn G Gri> 
+      neighbourhood_imp Gri v 
+    <\<lambda> r. graph_assn G Gri * is_neighb (\<N>\<^sub>G v) r>"
+    unfolding neighbourhood_imp_def graph_assn_def
+  apply(rule ht_bind[where R = "\<lambda> r. \<exists>\<^sub>AA. is_map A Gri * \<up> (finite (dom A)) * \<up> (dom (lookup G) = dom A) *
+           Finite_Set.fold (\<lambda>i. ( * ) (is_neighb (the (lookup G i)) (the (A i)))) emp (dom A) * \<up> (r = A v)"])
+  subgoal
+    by sep_auto
+  subgoal for nho
+    apply(clarsimp split!: option.split)
+    subgoal
+      apply(rule ht_ex_pre_and_post_I)
+      subgoal for A
+        apply(clarsimp split: option.split simp add:  Graph.neighbourhood_def)
+        using nd_emp_rule apply sep_auto
+        by force
+      done
+    subgoal for nh
+      apply(rule ht_ex_pre_and_post_I)
+      subgoal for A
+        apply(rule ht_cons_prec[where P' = 
+           "is_map A Gri * \<up> (finite (dom A)) * \<up> (dom (lookup G) = dom A) *
+    Finite_Set.fold (\<lambda>i. ( * ) (is_neighb (the (lookup G i)) (the (A i)))) emp (dom A - {v}) *
+    (is_neighb (the (lookup G v)) (the (A v))) *
+    \<up> (Some nh = A v)" and Q =
+       "\<lambda> x. (is_map A Gri * \<up> (finite (dom A)) * \<up> (dom (lookup G) = dom A) *
+    Finite_Set.fold (\<lambda>i. ( * ) (is_neighb (the (lookup G i)) (the (A i)))) emp (dom A - {v}) *
+    (is_neighb (the (lookup G v)) (the (A v))) *
+    \<up> (Some nh = A v)) * is_neighb (\<N>\<^sub>G v) x"])
+        subgoal
+          apply sep_auto
+          subgoal
+            apply(subst assn_over_finite_extract_one[of "dom A" v])
+            by sep_auto 
+          by sep_auto
+        subgoal for x
+          apply sep_auto
+          subgoal
+            apply(subst assn_over_finite_extract_one[of "dom A" v])
+             by sep_auto
+            by sep_auto 
+        subgoal
+        apply (sep_auto simp: Graph.neighbourhood_def split: option.split)
+         apply (metis domI domIff)
+        
+
+          find_theorems Finite_Set.fold "( * )"
+
+        
+
+    apply(rule ht_exEI)
+    subgoal for A
+      apply sep_auto
+      apply(rule ht_exPI[of _ _ _ A])
+      using imp_graph_map.lookup_rule[of A Gri]
+      apply sep_auto
+
+
+    find_theorems "<_> _ <\<lambda> _. \<exists>\<^sub>A _ . _ >"
+    apply sep_auto
+    subgoal for a b A
+      using imp_graph_map.lookup_rule[of A Gri]
+      
+    using assn_over_finite_extract_one[ of "dom A" 
+]
+  sorry
+*)
+
+lemma "<emp> do {x \<leftarrow> nh_emp; z \<leftarrow> nh_emp;  y \<leftarrow> if x = x then return y else undefined; return y} 
+       <\<lambda> r. \<up> (r = y)>"
+  using nd_emp_rule
+  by sep_auto
+ 
+
+lemma next_frontier_body_rule:
+   "<graph_assn G Gi  * is_vis vis visi * is_wfront nf nfi>
+     next_frontier_body Gi visi u nfi
+    <\<lambda> r. graph_assn G Gi * is_vis vis visi * is_wfront (nf \<union>\<^sub>G (diff (\<N>\<^sub>G u) vis)) r>"
+  unfolding next_frontier_body_def neighbourhood_imp_def
+            graph_assn_def ex_distrib_star[symmetric]
+  apply(rule ht_ex_pre_and_post_I)
+  subgoal for A
+    apply simp
+    apply(rule ht_bind[where R = "\<lambda> r. is_map A Gi * \<up> (finite (dom A)) * \<up> (dom (lookup G) = dom A) *
+     Finite_Set.fold (\<lambda>i. (*) (is_neighb (the (lookup G i)) (the (A i)))) emp (dom A) *
+     is_vis vis visi *
+     is_wfront nf nfi * \<up> (r = A u)"])
+    subgoal
+      by sep_auto
+    subgoal for nho
+      apply(clarsimp split!: option.split)
+      subgoal
+        apply(rule ht_bind[where R = "\<lambda> r. is_map A Gi * \<up> (finite (dom A)) * \<up> (dom (lookup G) = dom A) *
+     Finite_Set.fold (\<lambda>i. (*) (is_neighb (the (lookup G i)) (the (A i)))) emp (dom A) *
+     is_vis vis visi *
+     is_wfront nf nfi *
+     \<up> (A u = None) * is_neighb \<emptyset>\<^sub>N r"])
+        subgoal
+          using nd_emp_rule
+          by sep_auto
+        subgoal for empi
+        apply(rule ht_bind[where R = "\<lambda> r. is_map A Gi * \<up> (finite (dom A)) * \<up> (dom (lookup G) = dom A) *
+     Finite_Set.fold (\<lambda>i. (*) (is_neighb (the (lookup G i)) (the (A i)))) emp (dom A) *
+     is_vis vis visi *
+     is_wfront nf nfi *
+     \<up> (A u = None) *
+     is_neighb \<emptyset>\<^sub>N empi * is_neighb_nv (\<emptyset>\<^sub>N -\<^sub>G vis) r"])
+          subgoal
+            using unvisited_neighbs_rule by sep_auto
+          subgoal for nh_without_vis
+            using add_to_working_frontier_rule[of nf nfi "\<emptyset>\<^sub>N -\<^sub>G vis" nh_without_vis]
+            by (sep_auto simp: Graph.neighbourhood_def split: option.split)
+          done
+        done
+      subgoal for nho
+
+        apply(rule ht_cons_prec[where P' = "is_map A Gi * \<up> (finite (dom A)) * \<up> (dom (lookup G) = dom A) *
+     Finite_Set.fold (\<lambda>i. (*) (is_neighb (the (lookup G i)) (the (A i)))) emp (dom A - {u}) *
+     is_vis vis visi *
+     is_wfront nf nfi *
+     \<up> (A u = Some nho) 
+     *is_neighb (the (lookup G u)) (the (A u))"
+       and Q = "\<lambda> r. is_map A Gi * \<up> (finite (dom A)) * \<up> (dom (lookup G) = dom A) *
+         Finite_Set.fold (\<lambda>i. (*) (is_neighb (the (lookup G i)) (the (A i)))) emp (dom A - {u}) *
+         is_vis vis visi *is_neighb (the (lookup G u)) (the (A u)) * \<up> (Some nho = A u)*
+         is_wfront (nf \<union>\<^sub>G (\<N>\<^sub>G u -\<^sub>G vis)) r "])
+        subgoal
+          apply sep_auto
+          subgoal
+            apply(subst assn_over_finite_extract_one[of "dom A" u])
+            by sep_auto
+          by sep_auto
+        subgoal
+          apply sep_auto
+          subgoal
+            apply(subst assn_over_finite_extract_one[of "dom A" u])
+            by sep_auto
+          by sep_auto
+        apply(rule ht_bind[where R = "\<lambda> r. is_map A Gi * \<up> (finite (dom A)) * \<up> (dom (lookup G) = dom A) *
+     Finite_Set.fold (\<lambda>i. (*) (is_neighb (the (lookup G i)) (the (A i)))) emp (dom A - {u}) *
+     is_vis vis visi *
+     is_wfront nf nfi *
+     \<up> (A u = Some nho) *
+     is_neighb (the (lookup G u)) (the (A u)) * is_neighb_nv (the (lookup G u) -\<^sub>G vis) r"])
+        subgoal
+          using unvisited_neighbs_rule
+          by sep_auto
+        apply(cases "lookup G u")
+        subgoal
+          by sep_auto
+        unfolding Graph.neighbourhood_def
+        apply simp
+
+        using add_to_working_frontier_rule
+        by sep_auto
+      done
+    done
+  done
+
+lemma next_frontier_imperative_rule:
+   "<graph_assn G Gi * is_front frontier frontieri * is_vis vis visi> 
+     next_frontier_imperative Gi frontieri visi 
+    <\<lambda> r. graph_assn G Gi * is_front frontier frontieri * is_vis vis visi 
+          * is_front (next_frontier frontier vis) r >"
+  unfolding next_frontier_imperative_def
+  apply(rule ht_bind[where R = "\<lambda> r. graph_assn G Gi * is_front frontier frontieri * is_vis vis visi * is_wfront \<emptyset>\<^sub>N r"])
+  subgoal
+    using wf_empty_rule
+    by sep_auto
+  subgoal for empi
+    apply(rule ht_bind)
+     (*apply(rule ht_cons_prec)*)
+    apply(rule ht_cons_pre)
+    defer
+    apply(rule frontier_fold_rule[of "is_vis vis visi * graph_assn G Gi" "next_frontier_body Gi visi"
+                 "\<lambda> u frontier. frontier \<union>\<^sub>G (\<N>\<^sub>G u -\<^sub>G vis)" frontier frontieri "\<emptyset>\<^sub>N" "empi"])
+    subgoal  for u f fi
+      using next_frontier_body_rule[of Gi vis visi f fi u] by sep_auto
+    subgoal for new_wf
+      using to_ordinary_frontier_rule[of _  new_wf]
+      by(sep_auto simp: next_frontier_def)
+    subgoal
+      by sep_auto
+    done
+  done
+
+definition "dag_assn D Di = 
+  (\<exists>\<^sub>A A. is_dag A Di * \<up> (adjmap_inv D) * \<up> (finite (dom A)) *  \<up> (dom (lookup D) = dom A)*
+       Finite_Set.fold (\<lambda> i ass. is_dag_nh (the (lookup D i)) (the (A i)) * ass) emp (dom A))"
+
+lemma add_dag_neighbs_imp_rule:
+ "<dag_assn D Di * is_neighb_nv more_nh more_nhi>
+   add_dag_neighbs_imp Di u more_nhi
+  <\<lambda> r. dag_assn (add_neighbs D u more_nh) r * is_neighb_nv more_nh more_nhi>"
+  unfolding add_dag_neighbs_imp_def unfolding dag_assn_def ex_assn_move_out(1)
+  apply(rule ht_exEI)
+  subgoal for A
+    apply(rule ht_bind[where R = "\<lambda> r. is_dag A Di * \<up> (adjmap_inv D)* \<up> (finite (dom A)) * \<up> (dom (lookup D) = dom A) *
+     Finite_Set.fold (\<lambda>i. (*) (is_dag_nh (the (lookup D i)) (the (A i)))) emp (dom A) *
+     is_neighb_nv more_nh more_nhi  * \<up> (r = (more_nh = \<emptyset>\<^sub>N))"])
+    subgoal
+      using is_neighb_nv_emp_rule by sep_auto
+    subgoal for b
+      apply(clarsimp split!: if_split)
+      subgoal
+        by (sep_auto simp: add_neighbs_def)
+    apply(rule ht_bind[where R = "\<lambda> r. is_dag A Di * \<up> (adjmap_inv D)* \<up> (finite (dom A)) * \<up> (dom (lookup D) = dom A) *
+     Finite_Set.fold (\<lambda>i. (*) (is_dag_nh (the (lookup D i)) (the (A i)))) emp (dom A) *
+     is_neighb_nv more_nh more_nhi  * \<up> (r = A u) * \<up> (more_nh \<noteq> \<emptyset>\<^sub>N)"])
+    subgoal 
+      by sep_auto
+    subgoal for nhuo
+      apply(clarsimp split!: option.split)
+      subgoal
+        apply(rule ht_bind[where R = "\<lambda> r. is_dag A Di * \<up> (adjmap_inv D) * \<up> (finite (dom A)) * \<up> (dom (lookup D) = dom A) *
+     Finite_Set.fold (\<lambda>i. (*) (is_dag_nh (the (lookup D i)) (the (A i)))) emp (dom A) *
+     is_neighb_nv more_nh more_nhi *
+     \<up> (None = A u) * is_dag_nh more_nh r * \<up> (more_nh \<noteq> \<emptyset>\<^sub>N)"])
+        subgoal
+          using to_dag_nh_rule by sep_auto
+          subgoal
+            for new_dag_nh
+            apply(rule ht_exPI[of  _ _ _ "A(u\<mapsto>new_dag_nh)"])
+            using imp_dag_map_upd.update_rule[of A Di u new_dag_nh]
+            apply sep_auto
+            apply(subst assn_over_finite_insert_one)
+              apply simp
+             apply force
+            apply(subst assns_over_set_cong[where assn' = is_dag_nh
+              and f' = "\<lambda> i. the (lookup D i)" and g' = "the o A"])
+              apply simp
+            subgoal
+              by(auto simp add: add_neighbs_def Graph.adjmap.map_update split: option.split)
+            apply (sep_auto simp: add_neighbs_def Graph.adjmap.map_update Graph.adjmap.invar_update 
+                           split: option.split)
+            by force
+          done
+        subgoal for nhu
+          apply(rule ht_cons_pre[of _ "is_dag A Di * \<up> (adjmap_inv D) * \<up> (finite (dom A)) * \<up> (dom (lookup D) = dom A) *
+    Finite_Set.fold (\<lambda>i. (*) (is_dag_nh (the (lookup D i)) (the (A i)))) emp (dom A - {u}) *
+    is_neighb_nv more_nh more_nhi *
+    is_dag_nh (the (lookup D u)) nhu *
+    \<up> (A u = Some nhu ) *
+    \<up> (more_nh \<noteq> \<emptyset>\<^sub>N)"])
+          subgoal
+            apply sep_auto
+            subgoal
+              apply(subst assn_over_finite_extract_one[where i = u])
+                apply simp
+               apply force
+              apply sep_auto
+              by (smt (verit, best) assn_aci(11) entails_def option.sel)
+            by sep_auto
+          apply(rule ht_bind[where R = "\<lambda> r. is_dag A Di * \<up> (adjmap_inv D) * \<up> (finite (dom A)) * \<up> (dom (lookup D) = dom A) *
+     Finite_Set.fold (\<lambda>i. (*) (is_dag_nh (the (lookup D i)) (the (A i)))) emp (dom A - {u}) *
+     is_neighb_nv more_nh more_nhi *
+     is_dag_nh (the (lookup D u) \<union>\<^sub>G more_nh) r *
+     \<up> (A u = Some nhu) *
+     \<up> (more_nh \<noteq> \<emptyset>\<^sub>N)"])
+          subgoal
+            using  add_to_dag_nh_rule
+            by sep_auto
+          subgoal for bigger_nh
+            apply(rule ht_exPI[of _ _ _ "A(u \<mapsto> bigger_nh)"])
+            apply(rule ht_cons_post_prec[where Q = 
+     "\<lambda> r. is_dag (A(u \<mapsto> bigger_nh)) r * \<up> (adjmap_inv D) * 
+          \<up> (finite (dom (A(u \<mapsto> bigger_nh)))) *
+          \<up> (dom (lookup (add_neighbs D u more_nh)) = dom (A(u \<mapsto> bigger_nh))) *
+          Finite_Set.fold
+           (\<lambda>i. (*) (is_dag_nh (the (lookup D i)) (the ((A) i)))) emp
+           (dom A - {u}) * is_neighb_nv more_nh more_nhi
+         *is_dag_nh (the (lookup (add_neighbs D u more_nh) u)) bigger_nh * \<up> (more_nh \<noteq> \<emptyset>\<^sub>N)"])
+            subgoal
+              using imp_dag_map_upd.update_rule[of A Di u bigger_nh]
+              by (sep_auto simp: add_neighbs_def Graph.adjmap.map_update  Graph.adjmap.invar_update split: option.split)
+            subgoal for new_Gi
+              apply sep_auto
+              subgoal
+                apply(subst assn_over_finite_extract_one[where S = "Set.insert u (dom A)" and i = u])
+                  apply simp
+                 apply simp
+                apply simp
+                apply(subst (2) assns_over_set_cong[where assn' = is_dag_nh and f' = "\<lambda> i. (the (lookup D i))"
+                         and g'="the o A"])
+                  apply simp
+                subgoal
+                  by(auto simp add: add_neighbs_def Graph.adjmap.map_update split: option.split)
+                by sep_auto
+              by (sep_auto simp: add_neighbs_def Graph.adjmap.invar_update Graph.adjmap.map_update
+                          split: option.split)
+            done
+          done
+        done
+      done
+    done
+  done
+
+lemma expand_tree_body_rule:
+   "<graph_assn G Gi * is_vis vis visi * dag_assn D Di>
+     expand_tree_body Gi visi u Di
+    <\<lambda> r. graph_assn G Gi * is_vis vis visi * dag_assn (add_neighbs D u (\<N>\<^sub>G u -\<^sub>G vis)) r>"
+  unfolding expand_tree_body_def neighbourhood_imp_def
+            graph_assn_def ex_distrib_star[symmetric]
+  apply(rule ht_ex_pre_and_post_I)
+  subgoal for A
+    apply simp
+    apply(rule ht_bind[where R = "\<lambda> r. is_map A Gi * \<up> (finite (dom A)) * \<up> (dom (lookup G) = dom A) *
+     Finite_Set.fold (\<lambda>i. (*) (is_neighb (the (lookup G i)) (the (A i)))) emp (dom A) *
+     is_vis vis visi *
+     dag_assn D Di * \<up> (r = A u)"])
+    subgoal
+      by sep_auto
+    subgoal for nho
+      apply(clarsimp split!: option.split)
+      subgoal
+        apply(rule ht_bind[where R = "\<lambda> r. is_map A Gi * \<up> (finite (dom A)) * \<up> (dom (lookup G) = dom A) *
+     Finite_Set.fold (\<lambda>i. (*) (is_neighb (the (lookup G i)) (the (A i)))) emp (dom A) *
+     is_vis vis visi *
+     dag_assn D Di *
+     \<up> (None = A u) *
+     \<up> (A u = None) * is_neighb \<emptyset>\<^sub>N r"])
+        subgoal
+          using nd_emp_rule
+          by sep_auto
+        subgoal for empi
+        apply(rule ht_bind[where R = "\<lambda> r. is_map A Gi * \<up> (finite (dom A)) * \<up> (dom (lookup G) = dom A) *
+     Finite_Set.fold (\<lambda>i. (*) (is_neighb (the (lookup G i)) (the (A i)))) emp (dom A) *
+     is_vis vis visi *
+     dag_assn D Di *
+     \<up> (A u = None) *
+     is_neighb \<emptyset>\<^sub>N empi * is_neighb_nv (\<emptyset>\<^sub>N -\<^sub>G vis) r"])
+          subgoal
+            using unvisited_neighbs_rule by sep_auto
+          subgoal for nh_without_vis
+            using add_dag_neighbs_imp_rule[of D Di "\<emptyset>\<^sub>N -\<^sub>G vis" nh_without_vis u]
+            by (sep_auto simp: Graph.neighbourhood_def split: option.split)
+          done
+        done
+      subgoal for nho
+
+        apply(rule ht_cons_prec[where P' = "is_map A Gi * \<up> (finite (dom A)) * \<up> (dom (lookup G) = dom A) *
+     Finite_Set.fold (\<lambda>i. (*) (is_neighb (the (lookup G i)) (the (A i)))) emp (dom A - {u}) *
+     is_vis vis visi *
+     dag_assn D Di *
+     \<up> (A u = Some nho) 
+     *is_neighb (the (lookup G u)) (the (A u))"
+       and Q = "\<lambda> r. is_map A Gi * \<up> (finite (dom A)) * \<up> (dom (lookup G) = dom A) *
+         Finite_Set.fold (\<lambda>i. (*) (is_neighb (the (lookup G i)) (the (A i)))) emp (dom A - {u}) *
+         is_vis vis visi *is_neighb (the (lookup G u)) (the (A u)) * \<up> (Some nho = A u)*
+         dag_assn (add_neighbs D u (\<N>\<^sub>G u -\<^sub>G vis)) r "])
+        subgoal
+          apply sep_auto
+          subgoal
+            apply(subst assn_over_finite_extract_one[of "dom A" u])
+            by sep_auto
+          by sep_auto
+        subgoal
+          apply sep_auto
+          subgoal
+            apply(subst assn_over_finite_extract_one[of "dom A" u])
+            by sep_auto
+          by sep_auto
+        apply(rule ht_bind[where R = "\<lambda> r. is_map A Gi * \<up> (finite (dom A)) * \<up> (dom (lookup G) = dom A) *
+     Finite_Set.fold (\<lambda>i. (*) (is_neighb (the (lookup G i)) (the (A i)))) emp (dom A - {u}) *
+     is_vis vis visi *
+     dag_assn D Di *
+     \<up> (A u = Some nho) *
+     is_neighb (the (lookup G u)) (the (A u)) * is_neighb_nv (the (lookup G u) -\<^sub>G vis) r"])
+        subgoal
+          using unvisited_neighbs_rule
+          by sep_auto
+        apply(cases "lookup G u")
+        subgoal
+          by sep_auto
+        using add_dag_neighbs_imp_rule 
+        by (sep_auto simp: Graph.neighbourhood_def)
+      done
+    done
+  done
+
+lemma expand_tree_rule:
+   "<graph_assn G Gi * is_front front fronti * is_vis vis visi * dag_assn D Di>
+     expand_tree_imp Gi Di fronti visi
+    <\<lambda> r. graph_assn G Gi * is_front front fronti * is_vis vis visi * 
+           dag_assn (expand_tree D front vis) r>"
+  unfolding expand_tree_imp_def expand_tree_def
+  using expand_tree_body_rule[of Gi vis visi]
+  using dag_fold_imp[of "graph_assn G Gi * is_vis vis visi" dag_assn  "expand_tree_body Gi visi"  ] 
+  by sep_auto
+
+
+lemma dag_empty_rule:
+ "<emp>dag_empty<dag_assn empty>"
+  unfolding dag_assn_def
+  by(rule ht_exPI[where x = "\<lambda> x. None"])
+    (sep_auto simp: Graph.adjmap.invar_empty Graph.adjmap.map_empty)
+
+end
+
+end 
