Set_Graphs/Graph_Algorithms/BFS_Refinement_Instantiation.thy
@@ -1,0 +1,618 @@
+theory BFS_Refinement_Instantiation
+  imports BFS_Refinement
+begin
+
+definition "list_union xs ys = fold (\<lambda> y ys. if y \<in> set ys then ys else y#ys) ys xs"
+
+fun list_union' where
+ "list_union' xs Nil = xs" |
+ "list_union' xs (y#ys) = (if y \<in> set ys then list_union' xs ys else y#list_union' xs ys)"
+
+lemma list_union'_is:
+  "list_union' xs ys = remdups ys @ xs"
+  by(induction ys) auto
+
+lemma list_union_set_rev:"set (list_union xs (rev ys)) = set xs \<union> set ys"
+  unfolding list_union_def
+  unfolding foldr_conv_fold[symmetric]
+  by(induction ys) auto
+
+lemma list_union_set:"set (list_union xs ys) = set xs \<union> set ys"
+  using list_union_set_rev[of xs "rev ys"] by simp
+
+lemma list_union_distinct_rev:"\<lbrakk>distinct xs; distinct ys\<rbrakk> \<Longrightarrow> distinct (list_union xs (rev ys))"
+  unfolding list_union_def
+  unfolding foldr_conv_fold[symmetric]
+  by(induction ys) auto
+
+lemma list_union_distinct:"\<lbrakk>distinct xs; distinct ys\<rbrakk> \<Longrightarrow> distinct (list_union xs ys)"
+  using list_union_distinct_rev[of xs "rev ys"] by simp
+
+definition "is_front xs xsi = \<up> (xs = xsi)"
+
+definition "imp_cf_is_empty xs = return (xs = Nil)"
+
+lemma imp_cf_is_empty_rule:
+  "<is_front S Si> imp_cf_is_empty Si <\<lambda>b. is_front S Si * \<up> (b = (S = []))>"
+  by(sep_auto simp: imp_cf_is_empty_def is_front_def)
+
+locale guarded_list =
+imp_set_ins +
+imp_set_memb +
+imp_set_empty
+begin
+
+fun guarded_list_assn where 
+"guarded_list_assn xs (S, xsi) = 
+  is_set (set xs) S * \<up> (xs = xsi) * \<up> (distinct xsi)"
+
+definition "guarded_list_empty = do {i \<leftarrow> empty; return (i, Nil)}"
+
+lemma guarded_list_empty_rule:
+  "<emp> guarded_list_empty <guarded_list_assn Nil>"
+  by(sep_auto simp: guarded_list_empty_def)
+
+fun add_one_to_guarded_list where
+ "add_one_to_guarded_list x (S, xsi) =
+   do{b \<leftarrow> memb x S;
+      if b then return (S, xsi)
+      else do{
+         S' \<leftarrow> ins x S;
+         return (S', x#xsi)}}"
+
+lemma add_one_to_guarded_list_rule:
+ "<guarded_list_assn xs S>
+   add_one_to_guarded_list x S
+ <\<lambda> S. guarded_list_assn (if x \<in> set xs then xs else x#xs) S>"
+  by(cases S) sep_auto
+
+definition "add_all_to_guarded_list S xs = 
+  foldM add_one_to_guarded_list xs S"
+
+lemma add_all_to_guarded_list_rule:
+  "<guarded_list_assn xs S>
+   add_all_to_guarded_list S ys
+ <\<lambda> S. guarded_list_assn (list_union xs ys) S>"
+  unfolding add_all_to_guarded_list_def list_union_def
+  apply(rule foldM_refine[where fi = add_one_to_guarded_list and xs = ys and si = S
+            and f = "\<lambda>y ys. if y \<in> set ys then ys else y # ys" 
+             and I = "\<lambda> _ _. guarded_list_assn"])
+  using add_one_to_guarded_list_rule
+  by sep_auto
+
+fun to_ordinary_list where
+ "to_ordinary_list (S, xs) = return xs"
+
+lemma to_ordinary_list_rule:
+  "<guarded_list_assn xs S>
+    to_ordinary_list S
+   <\<lambda> r. guarded_list_assn xs S * \<up>(r = xs)>"
+  by(cases S) sep_auto
+
+definition to_guarded_list where
+ "to_guarded_list xs =
+  do {i \<leftarrow> empty;
+      S \<leftarrow> foldM ins xs i;
+      return (S, xs)}"
+
+lemma foldM_ins: "<is_set S Si>foldM ins xs Si <is_set (S \<union> set xs)>"
+proof-
+  have  "<is_set S Si>foldM ins xs Si <is_set (fold Set.insert xs S)>"
+    using foldM_refine[of "\<lambda> a b. is_set" xs ins Set.insert S Si]
+    by sep_auto
+  moreover have "fold Set.insert xs S =  S \<union> set xs"
+    using union_set_fold[of xs] by auto
+  ultimately show ?thesis
+    by simp
+qed
+
+lemma to_guarded_list_rule:
+ "<\<up> (distinct xs)> to_guarded_list xs <\<lambda> r. guarded_list_assn xs r>"
+  unfolding to_guarded_list_def
+  using foldM_ins
+  by sep_auto
+
+end
+
+locale list_set_diff = imp_set_memb
+begin
+
+fun list_cleared_of_set where
+  "list_cleared_of_set Nil S = return Nil" |
+  "list_cleared_of_set (x#xs) S =
+    do {b \<leftarrow> memb x S;
+        if b 
+        then list_cleared_of_set xs S
+        else do {rest \<leftarrow> list_cleared_of_set xs S;
+                 return (x#rest)}}"
+
+lemma list_cleared_of_set_rule:
+  "<is_set S Si * \<up> (distinct xs)> list_cleared_of_set xs Si 
+   <\<lambda> r. is_set S Si * \<up> (distinct r) * \<up> (r = filter (\<lambda> x. x \<notin> S) xs)>"
+  by(induction xs) sep_auto
+
+end
+
+locale add_list_to_a_set = imp_set_ins
+begin
+
+definition "add_list_to_set xs S= foldM ins xs S"
+
+end
+
+
+(*
+setup Locale_Code.open_block 
+interpretation hash_guarded_list: guarded_list is_hashset hs_ins hs_memb hs_new
+  by unfold_locales
+setup Locale_Code.close_block 
+*)
+
+locale list_array_map_based_bfs = 
+imp_set_ins is_set1 ins1 +
+imp_set_memb is_set1 memb1+
+imp_set_empty is_set1 empty1 +
+imp_set_memb is_set2 memb2 +
+imp_set_ins is_set2 ins2 +
+imp_set_empty is_set2 empty2 +
+imp_set_memb is_set3 memb3 +
+imp_set_ins is_set3 ins3 +
+imp_set_empty is_set3 empty3 +
+imp_map_lookup is_map lookup_imp +
+imp_map_lookup is_dag lookup_dag_imp +
+imp_map_update is_dag update_dag_imp +
+imp_map_empty is_dag dag_empty 
+for is_set1:: "'v set \<Rightarrow> 'nset \<Rightarrow> assn" and ins1 memb1 empty1 
+and is_set2 :: "'v set \<Rightarrow> 'vis \<Rightarrow> assn" and memb2
+and is_set3 :: "'v set \<Rightarrow> 'dag_nh_set \<Rightarrow> assn" and memb3 and ins3 and empty3
+and is_map::"('v \<Rightarrow> 'v list option) \<Rightarrow> 'g_array \<Rightarrow> assn" and  lookup_imp
+and is_dag :: "('v \<Rightarrow> ('dag_nh_set \<times> 'v list) option) \<Rightarrow> 'a \<Rightarrow> assn"
+and lookup_dag_imp update_dag_imp dag_empty empty2 ins2
+begin
+
+interpretation guarded_list is_set1 ins1 memb1 empty1
+  by unfold_locales
+
+abbreviation "gl_empty \<equiv> guarded_list_empty"
+abbreviation "gl_assn \<equiv> guarded_list_assn"
+
+definition "nh_emp = return Nil"
+definition "is_neighb xs xsi = \<up> (xs = xsi) * \<up> (distinct xs)"
+
+definition "is_neighb_nv xs xsi = \<up> (xs = xsi) * \<up> (distinct xs)"
+definition "is_neighb_nv_emp xsi = return (xsi = Nil)"
+
+interpretation list_set_diff is_set2 memb2
+  by unfold_locales
+
+definition "is_vis xs S = is_set2 (set xs) S"
+
+definition "vis_empty = empty2"
+
+lemma vis_empty_rule: "<emp> vis_empty <is_vis []>"
+  by(sep_auto simp: is_vis_def vis_empty_def)
+
+definition "imp_src_to_cf xs = return xs"
+
+definition "imp_src_assn S Si = \<up> (S = Si)"
+
+lemma imp_src_to_cf_rule:  
+  "<imp_src_assn S Si> imp_src_to_cf Si <\<lambda>r. imp_src_assn S Si * is_front S r>"
+  by(sep_auto simp: imp_src_assn_def imp_src_to_cf_def is_front_def)
+
+find_theorems "_::'vis"
+
+definition "set_cf_visited imp_vis imp_cf = foldM ins2 imp_cf imp_vis"
+
+lemma set_cf_visited_rule:
+   "<is_vis vis imp_vis * is_front cf imp_cf> set_cf_visited imp_vis imp_cf
+    <\<lambda>r. is_vis (list_union vis cf) r * is_front cf imp_cf>"
+  unfolding set_cf_visited_def list_union_def
+  apply(rule ht_cons_prec[rotated, rotated])
+  apply(rule foldM_refine[where fi = ins2 and xs = imp_cf and si = imp_vis 
+         and f = "\<lambda>y ys. if y \<in> set ys then ys else y # ys" and s = vis
+      and I = "\<lambda> _ _ vis imp_vis. is_vis vis imp_vis * is_front cf imp_cf"])
+  subgoal for xs\<^sub>1 x xs\<^sub>2 s si
+    by(sep_auto simp: is_vis_def is_front_def insert_absorb)
+  subgoal
+    by sep_auto
+  subgoal for x
+    by (sep_auto simp: is_front_def)
+  done
+
+interpretation dag_nh: guarded_list is_set3 ins3 memb3 empty3
+  by unfold_locales
+
+interpretation subprocedures: BFS_subprocedures_Imperative
+  where empty = "\<lambda> x. None"
+  and delete = "\<lambda> x M y. if y = x then None else M y"
+  and update =  "\<lambda> x y M. M (x\<mapsto> y)"
+  and adjmap_inv = "\<lambda> x. True"
+  and lookup = "\<lambda> M x. M x"
+  and G = G
+  and vset_empty = Nil
+  and vset_delete = "\<lambda> x xs. filter (\<lambda> y. y\<noteq> x) xs"
+  and vset_inv = distinct
+  and union = list_union
+  and inter = "\<lambda> xs ys. filter (\<lambda> y. y \<in> set xs) ys"
+  and insert = "\<lambda> x xs. if x \<in> set xs then xs else x#xs"
+  and diff = "\<lambda> xs ys. filter (\<lambda> y. y \<notin> set ys) xs"
+  and fold_vset = fold
+  and fold_adjmap = fold
+  and isin = "\<lambda> xs x. x \<in> set xs"
+  and t_set = set
+  and sel = hd
+  and dag_fold_imp = foldM
+  and is_front = is_front
+  and frontier_fold_imp = foldM
+  and is_wfront = gl_assn
+  and wf_empty = gl_empty
+  and nh_emp = nh_emp
+  and is_neighb = is_neighb
+  and is_neighb_nv = is_neighb_nv
+  and is_neighb_nv_emp= is_neighb_nv_emp
+  and unvisited_neighbs=list_cleared_of_set
+  and is_vis = is_vis
+  and add_to_working_frontier = add_all_to_guarded_list
+  and to_ordinary_frontier = to_ordinary_list
+  and add_to_dag_nh = dag_nh.add_all_to_guarded_list
+  and is_dag_nh = dag_nh.guarded_list_assn
+  and to_dag_nh = dag_nh.to_guarded_list
+  and lookup_imp = lookup_imp
+  and is_map = is_map
+  and is_dag = is_dag
+  and lookup_dag_imp = lookup_dag_imp
+  and update_dag_imp = update_dag_imp
+  and dag_empty = dag_empty
+for G :: "'v \<Rightarrow> 'v list option"
+proof(rule BFS_subprocedures_Imperative.intro, goal_cases)
+  case 1
+  then show ?case 
+    by(auto intro!: BFS_subprocedures.intro Pair_Graph_Sepcs_Set2.intro
+                    Pair_Graph_Specs.intro Map.intro  Set_Choose.intro Set.intro
+                    Set_Choose_axioms.intro Set2.intro 
+                    Set2_axioms.intro BFS_subprocedures_axioms.intro exI[of _ "rev _"] 
+          simp add: foldr_conv_fold if_split[of "\<lambda> x. _ \<in> set x"] list_union_set list_union_distinct) 
+next
+  case 2
+  then show ?case
+    by unfold_locales
+next
+  case 3
+  then show ?case 
+   by unfold_locales
+next
+  case 4
+  then show ?case 
+   by unfold_locales
+next
+  case 5
+  then show ?case 
+    by unfold_locales
+next
+  case 6
+  thus ?case
+  proof(rule BFS_subprocedures_Imperative_axioms.intro, goal_cases)
+    case 1
+    then show ?case 
+      by(sep_auto simp: nh_emp_def is_neighb_def)
+  next
+    case 2
+    then show ?case
+      using guarded_list_empty_rule by simp
+  next
+    case (3 nnh nnhi)
+    then show ?case 
+      by(sep_auto simp: is_neighb_nv_def is_neighb_nv_emp_def)
+  next
+    case (4 nnh nnhi)
+    then show ?case 
+      by(simp add: is_neighb_nv_def)
+  next
+    case (5 nd ndi vis visi)
+    then show ?case
+      using list_cleared_of_set_rule[of "set vis" visi nd]
+      by(sep_auto simp: is_neighb_nv_def is_vis_def is_neighb_def)
+  next
+    case (6 f fi nh nhi)
+    then show ?case 
+      using add_all_to_guarded_list_rule[of f fi nhi]
+      by(sep_auto simp: is_neighb_nv_def)
+  next
+    case (7 front fronti init initi F fi f)
+    have "<F * is_front front fronti * gl_assn init initi> foldM fi fronti initi
+  <\<lambda>si. F * is_front front fronti * gl_assn (fold f fronti init) si>"
+      apply(rule foldM_refine[where fi = fi and f = f and xs = fronti and si = initi and s = init
+            and I = "\<lambda> a b x xi.  F * is_front front fronti * gl_assn x xi"])
+      subgoal for xs\<^sub>1 x xs\<^sub>2 s si
+        using 7[of s si x] by sep_auto
+      done
+    thus ?case
+      by(sep_auto simp: is_front_def)
+  next
+    case (8 f wfi)
+    then show ?case 
+      using to_ordinary_list_rule
+      by(sep_auto simp: is_front_def)
+  next
+    case (9 dag_nh dag_nhi nnh nnhi)
+    then show ?case
+      using dag_nh.add_all_to_guarded_list_rule
+      by(cases dag_nhi)(sep_auto simp: is_neighb_nv_def)
+  next
+    case (10 nh nhi)
+    then show ?case
+      using dag_nh.to_guarded_list_rule
+      by(sep_auto simp: is_neighb_nv_def)
+  next
+    case (11 front fronti init initi dag_assn F fi f)
+    have "<F * is_front front fronti * dag_assn init initi> foldM fi front initi
+      <\<lambda>si. F * is_front front fronti * dag_assn (fold f front init) si>"
+      apply(rule foldM_refine[where fi= fi and xs = front and si = initi and f= f and s = init
+             and I = "\<lambda> a b dag dagi. F * is_front front fronti * dag_assn dag dagi"])
+      subgoal for xs\<^sub>1 x xs\<^sub>2 s si
+        using 11[of s si x] by sep_auto
+      done
+    thus ?case
+      by(sep_auto simp: is_front_def)
+  qed
+qed
+
+interpretation bfs_imp: BFS_Imperative
+  where  empty = "\<lambda> x. None"
+  and delete = "\<lambda> x M y. if y = x then None else M y"
+  and update =  "\<lambda> x y M. M (x\<mapsto> y)"
+  and adjmap_inv = "\<lambda> x. True"
+  and lookup = "\<lambda> M x. M x"
+  and G = G
+  and vset_empty = Nil
+  and vset_delete = "\<lambda> x xs. filter (\<lambda> y. y\<noteq> x) xs"
+  and vset_inv = distinct
+  and union = list_union
+  and inter = "\<lambda> xs ys. filter (\<lambda> y. y \<in> set xs) ys"
+  and insert = "\<lambda> x xs. if x \<in> set xs then xs else x#xs"
+  and diff = "\<lambda> xs ys. filter (\<lambda> y. y \<notin> set ys) xs"
+  and isin = "\<lambda> xs x. x \<in> set xs"
+  and t_set = set
+  and sel = hd
+  and next_frontier = "subprocedures.next_frontier G"
+  and imp_dag_empty = dag_empty
+  and expand_tree = "subprocedures.expand_tree G"
+  and graph_assn = subprocedures.graph_assn
+  and imp_vis_empty = vis_empty
+  and set_cf_visited = set_cf_visited
+  and imp_expand_tree = "subprocedures.expand_tree_imp Gi"
+  and imp_next_frontier = "subprocedures.next_frontier_imperative Gi"
+  and imp_cf_is_empty = imp_cf_is_empty
+  and imp_dag_assn = subprocedures.dag_assn
+  and imp_vis_assn = is_vis
+  and imp_cf_assn = is_front
+  and imp_src_to_cf = imp_src_to_cf
+  and imp_src_assn = imp_src_assn 
+  and G_imp = Gi
+  and srcs = srcs
+for Gi G srcs
+proof(rule BFS_Imperative.intro, goal_cases)
+  case 1
+  then show ?case 
+    by(intro BFS.intro subprocedures.Graph.Pair_Graph_Specs_axioms
+             subprocedures.set_ops.Set2_axioms BFS_axioms.intro 
+             subprocedures.expand_tree subprocedures.next_frontier 
+      | assumption)+
+next
+  case 2
+  then show ?case 
+  proof(rule BFS_Imperative_axioms.intro, goal_cases)
+    case 1
+    then show ?case 
+      using subprocedures.dag_empty_rule by simp
+  next
+    case 2
+    then show ?case
+      using vis_empty_rule by simp
+  next
+    case (3 S Si)
+    then show ?case 
+      using imp_cf_is_empty_rule by auto
+  next
+    case (4 S Si)
+    then show ?case 
+      using imp_src_to_cf_rule[of S Si] by auto
+  next
+    case (5 vis imp_vis cf imp_cf)
+    then show ?case
+      using set_cf_visited_rule by simp
+  next
+    case (6 dag imp_dag cf imp_cf vis imp_vis)
+    then show ?case 
+      using subprocedures.expand_tree_rule[of G Gi cf imp_cf vis imp_vis dag imp_dag] 
+      by sep_auto
+  next
+    case (7 cf imp_cf vis imp_vis)
+    then show ?case 
+      using subprocedures.next_frontier_imperative_rule[of G Gi cf imp_cf vis imp_vis]
+      by sep_auto
+  qed
+qed
+
+lemmas BFS_refine = bfs_imp.BFS_refine
+lemmas graph_assn_def = subprocedures.graph_assn_def
+abbreviation "state_assn \<equiv> bfs_imp.state_assn"
+
+abbreviation "BFS_imp \<equiv> bfs_imp.BFS_imp"
+abbreviation "BFS_fun \<equiv> bfs_imp.BFS_impl"
+
+find_theorems  BFS.BFS_impl
+
+find_theorems subprocedures.expand_tree
+find_theorems BFS_subprocedures.expand_tree
+
+
+lemma "BFS_fun = 
+  (\<lambda> G. BFS.BFS_impl Nil list_union (subprocedures.expand_tree G)
+                  (subprocedures.next_frontier G))"
+  by simp
+
+term is_set1
+term is_set2
+term is_set3
+term empty2
+term ins2
+term lookup_imp
+end
+(*
+definition "ias_is_empty S = do {s \<leftarrow> Array.len S;
+                                 return (s = 0)}"
+
+
+interpretation imp_set_is_empty is_ias ias_is_empty
+  apply unfold_locales
+  apply(sep_auto simp: is_ias_def ias_of_list_def ias_is_empty_def)
+ *)
+
+setup Locale_Code.open_block 
+interpretation hash_guarded_list: guarded_list is_hashset hs_ins hs_memb hs_new
+  by unfold_locales
+
+interpretation visited_set_diff: list_set_diff is_ias ias_memb
+  by unfold_locales
+
+abbreviation "gl_empty \<equiv> hash_guarded_list.guarded_list_empty"
+definition "nh_emp = return Nil"
+definition "is_neighb_nv_emp xsi = return (xsi = Nil)"
+
+definition "vis_empty = ias_new"
+
+definition "imp_src_to_cf xs = return xs"
+
+definition "set_cf_visited imp_vis imp_cf = foldM ias_ins imp_cf imp_vis"
+
+interpretation subprocedures: BFS_subprocedures_Imperative_spec
+  where dag_fold_imp = foldM
+  and frontier_fold_imp = foldM
+  and wf_empty = gl_empty
+  and nh_emp = nh_emp
+  and is_neighb_nv_emp= is_neighb_nv_emp
+  and unvisited_neighbs= visited_set_diff.list_cleared_of_set
+  and add_to_working_frontier = hash_guarded_list.add_all_to_guarded_list
+  and to_ordinary_frontier = hash_guarded_list.to_ordinary_list
+  and add_to_dag_nh = hash_guarded_list.add_all_to_guarded_list
+  and to_dag_nh = hash_guarded_list.to_guarded_list
+  and lookup_imp = iam_lookup
+  and lookup_dag_imp = iam_lookup
+  and update_dag_imp = iam_update
+  done
+
+interpretation top_loop: BFS_Imperative_spec
+  where imp_dag_empty = iam_new
+  and imp_vis_empty = vis_empty
+  and set_cf_visited = set_cf_visited
+  and imp_expand_tree = "subprocedures.expand_tree_imp Gi"
+  and imp_next_frontier = "subprocedures.next_frontier_imperative Gi"
+  and imp_cf_is_empty = imp_cf_is_empty
+  and imp_src_to_cf = imp_src_to_cf for Gi
+  done
+
+interpretation iam_graph: Pair_Graph_Imperative  
+    is_iam iam_new iam_lookup iam_update 
+    by unfold_locales
+
+setup Locale_Code.close_block
+
+definition "BFS_imp = top_loop.BFS_imp"
+definition "initial_state = top_loop.initial_state_imp"
+definition "iam_graph_from_list = iam_graph.from_list_impl"
+
+thm top_loop.initial_state_imp_def
+thm top_loop.BFS_imp.simps
+(*
+export_code BFS_imp imp_src_to_cf iam_new vis_empty
+
+in SML_imp module_name exported file_prefix BFS_imperative
+*)
+ML_val \<open>
+val noi = @{code nat_of_integer}
+val graph_from_list = @{code iam_graph_from_list} o map (apply2 noi)
+val G = graph_from_list [(1,2), (2,3), (3,4), (3,5), (10,8), (11,12),
+    (1,10), (1,11), (1,12), (4,13), (5,1)] ()
+val initial_state = @{code initial_state} [noi 1] ()
+val bfs = @{code BFS_imp}
+val final_state = bfs G initial_state ()
+\<close>
+
+interpretation proofs: list_array_map_based_bfs
+   (*aux set for frontier building*)
+   is_hashset hs_ins hs_memb hs_new
+   (*visited*)
+   is_ias ias_memb
+   (*aux set for building dag nh*)
+   is_hashset hs_memb hs_ins hs_new
+   (*map for actual graph*)
+   is_iam iam_lookup
+   (**map for dag*)
+   is_iam iam_lookup iam_update iam_new 
+   (*visited part 2*)
+   ias_new ias_ins
+  by unfold_locales
+
+find_theorems proofs.BFS_imp
+find_theorems top_loop.BFS_imp
+
+abbreviation "bfs_graph_assn \<equiv> BFS_subprocedures_Imperative.graph_assn"
+abbreviation "state_assn \<equiv> BFS_Imperative.state_assn"
+abbreviation "bfs_loop \<equiv> BFS_Imperative_spec.BFS_imp"
+
+thm proofs.BFS_refine
+thm iam_graph.from_list_impl_rule
+
+lemma "bfs_graph_assn (\<lambda>M. M) is_iam proofs.is_neighb = iam_graph.finite_graph_assn"
+  apply(rule ext)+
+  unfolding proofs.graph_assn_def
+  unfolding iam_graph.finite_graph_assn_def
+  unfolding iam_graph.graph_inv_def
+  unfolding proofs.is_neighb_def
+  subgoal for amap map
+    apply(rule ent_iffI)
+
+     apply sep_auto
+    subgoal
+      apply(rule ent_ex_preI)
+      subgoal for A
+        apply sep_auto
+        subgoal
+          apply(sep_auto simp: pure_assn_over_finite_set)
+          apply(rule forw_subst[where P = "\<lambda> m. _ \<Longrightarrow>\<^sub>A is_iam m map" and b = A])
+          subgoal
+            apply(rule ext)
+            subgoal for x 
+              by(cases "amap x", all \<open>cases "A x"\<close>) force+
+            done
+          by simp
+        done
+      done
+    subgoal for a b v vset
+      apply (sep_auto simp: pure_assn_over_finite_set)
+      by force
+    subgoal
+     by (sep_auto simp: pure_assn_over_finite_set)
+    subgoal
+      apply(rule ent_ex_postI[of _ _ amap])
+      by (sep_auto simp: pure_assn_over_finite_set)
+    done
+  done
+
+lemma BFS_imp_def': "BFS_imp = proofs.BFS_imp"
+  unfolding BFS_imp_def is_neighb_nv_emp_def nh_emp_def proofs.is_neighb_nv_emp_def
+      proofs.nh_emp_def proofs.set_cf_visited_def set_cf_visited_def
+  by simp
+
+lemma BFS_imp_rule:
+"<bfs_graph_assn (\<lambda>M. M) is_iam proofs.is_neighb G Gi * proofs.state_assn s s_imp>
+BFS_imp Gi s_imp
+<\<lambda>s_imp'. bfs_graph_assn (\<lambda>M. M) is_iam proofs.is_neighb G Gi *
+    proofs.state_assn (proofs.BFS_fun G s) s_imp'>"
+  unfolding BFS_imp_def'
+  using proofs.BFS_refine
+  by simp
+
+end
